<?xml version="1.0"?>
<rdf:RDF xmlns="http://purl.obolibrary.org/obo/omrse/imports/oostt_import.owl#"
     xml:base="http://purl.obolibrary.org/obo/omrse/imports/oostt_import.owl"
     xmlns:dc="http://purl.org/dc/elements/1.1/"
     xmlns:obo="http://purl.obolibrary.org/obo/"
     xmlns:owl="http://www.w3.org/2002/07/owl#"
     xmlns:rdf="http://www.w3.org/1999/02/22-rdf-syntax-ns#"
     xmlns:xml="http://www.w3.org/XML/1998/namespace"
     xmlns:xsd="http://www.w3.org/2001/XMLSchema#"
     xmlns:rdfs="http://www.w3.org/2000/01/rdf-schema#">
    <owl:Ontology rdf:about="http://purl.obolibrary.org/obo/omrse/imports/oostt_import.owl">
        <owl:versionIRI rdf:resource="http://purl.obolibrary.org/obo/omrse/releases/2021-02-16/imports/oostt_import.owl"/>
        <dc:source rdf:resource="http://purl.obolibrary.org/obo/oostt//2021-01-08/oostt.owl"/>
        <owl:versionInfo rdf:datatype="http://www.w3.org/2001/XMLSchema#string">2021-02-16</owl:versionInfo>
    </owl:Ontology>
    


    <!-- 
    ///////////////////////////////////////////////////////////////////////////////////////
    //
    // Annotation properties
    //
    ///////////////////////////////////////////////////////////////////////////////////////
     -->

    


    <!-- http://purl.obolibrary.org/obo/IAO_0000115 -->

    <owl:AnnotationProperty rdf:about="http://purl.obolibrary.org/obo/IAO_0000115"/>
    


    <!-- http://purl.obolibrary.org/obo/IAO_0000117 -->

    <owl:AnnotationProperty rdf:about="http://purl.obolibrary.org/obo/IAO_0000117"/>
    


    <!-- http://purl.obolibrary.org/obo/IAO_0000119 -->

    <owl:AnnotationProperty rdf:about="http://purl.obolibrary.org/obo/IAO_0000119"/>
    


    <!-- http://purl.obolibrary.org/obo/OOSTT_00000030 -->

    <owl:AnnotationProperty rdf:about="http://purl.obolibrary.org/obo/OOSTT_00000030">
        <obo:IAO_0000117 xml:lang="en">Mathias Brochhausen</obo:IAO_0000117>
        <rdfs:label xml:lang="en">OOSTT user-centered description</rdfs:label>
    </owl:AnnotationProperty>
    


    <!-- 
    ///////////////////////////////////////////////////////////////////////////////////////
    //
    // Classes
    //
    ///////////////////////////////////////////////////////////////////////////////////////
     -->

    


    <!-- http://purl.obolibrary.org/obo/IAO_0000030 -->

    <owl:Class rdf:about="http://purl.obolibrary.org/obo/IAO_0000030"/>
    


    <!-- http://purl.obolibrary.org/obo/OOSTT_00000074 -->

    <owl:Class rdf:about="http://purl.obolibrary.org/obo/OOSTT_00000074">
        <rdfs:subClassOf rdf:resource="http://purl.obolibrary.org/obo/IAO_0000030"/>
        <obo:IAO_0000115 xml:lang="en">An information content entity that is the specified outcome of and documents the sucessful completion of a tertiary education program.</obo:IAO_0000115>
        <obo:IAO_0000117 xml:lang="en">John Judkins</obo:IAO_0000117>
        <obo:IAO_0000117 xml:lang="en">Mathias Brochhausen</obo:IAO_0000117>
        <obo:OOSTT_00000030 xml:lang="en">Recognized degree awarded after successful completion of a college or post-graduate porgram.</obo:OOSTT_00000030>
        <rdfs:label xml:lang="en">academic degree</rdfs:label>
    </owl:Class>
    


    <!-- http://purl.obolibrary.org/obo/OOSTT_00000081 -->

    <owl:Class rdf:about="http://purl.obolibrary.org/obo/OOSTT_00000081">
        <rdfs:subClassOf rdf:resource="http://purl.obolibrary.org/obo/OOSTT_00000074"/>
        <obo:IAO_0000115 xml:lang="en">An academic degree awarded by colleges and universities upon completion of a program of study lasting two years.</obo:IAO_0000115>
        <obo:IAO_0000117 xml:lang="en">John Judkins</obo:IAO_0000117>
        <obo:IAO_0000117 xml:lang="en">Mathias Brochhausen</obo:IAO_0000117>
        <obo:IAO_0000119 xml:lang="en">https://en.wikipedia.org/w/index.php?title=Associate_degree&amp;oldid=723897149</obo:IAO_0000119>
        <obo:OOSTT_00000030 xml:lang="en">Recognition awarded after completion of a specific curriculum from an accredited tertiary education provider that falls between high school and bachelor&apos;s degree program.</obo:OOSTT_00000030>
        <rdfs:label xml:lang="en">associate degree</rdfs:label>
    </owl:Class>
    


    <!-- http://purl.obolibrary.org/obo/OOSTT_00000082 -->

    <owl:Class rdf:about="http://purl.obolibrary.org/obo/OOSTT_00000082">
        <rdfs:subClassOf rdf:resource="http://purl.obolibrary.org/obo/OOSTT_00000074"/>
        <obo:IAO_0000115 xml:lang="en">An academic degree awarded by universities upon completion of a course of study demonstrating a mastery or high-order overview of a specific field of study or area of professional practice.[1] Within the area studied, graduates are posited to possess advanced knowledge of a specialized body of theoretical and applied topics; high order skills in analysis, critical evaluation, or professional application; and the ability to solve complex problems and think rigorously and independently.</obo:IAO_0000115>
        <obo:IAO_0000117 xml:lang="en">John Judkins</obo:IAO_0000117>
        <obo:IAO_0000117 xml:lang="en">Mathias Brochhausen</obo:IAO_0000117>
        <obo:IAO_0000119 xml:lang="en">https://en.wikipedia.org/w/index.php?title=Master%27s_degree&amp;oldid=726036185</obo:IAO_0000119>
        <rdfs:label xml:lang="en">master&apos;s degree</rdfs:label>
    </owl:Class>
    


    <!-- http://purl.obolibrary.org/obo/OOSTT_00000083 -->

    <owl:Class rdf:about="http://purl.obolibrary.org/obo/OOSTT_00000083">
        <rdfs:subClassOf rdf:resource="http://purl.obolibrary.org/obo/OOSTT_00000074"/>
        <obo:IAO_0000115 xml:lang="en">An academic degree awarded by colleges and universities upon completion of a course of study lasting three to seven years.</obo:IAO_0000115>
        <obo:IAO_0000117 xml:lang="en">John Judkins</obo:IAO_0000117>
        <obo:IAO_0000117 xml:lang="en">Mathias Brochhausen</obo:IAO_0000117>
        <obo:IAO_0000119 xml:lang="en">https://en.wikipedia.org/w/index.php?title=Bachelor%27s_degree&amp;oldid=725713923</obo:IAO_0000119>
        <rdfs:label xml:lang="en">bachelor&apos;s degree</rdfs:label>
    </owl:Class>
    


    <!-- http://purl.obolibrary.org/obo/OOSTT_00000084 -->

    <owl:Class rdf:about="http://purl.obolibrary.org/obo/OOSTT_00000084">
        <rdfs:subClassOf rdf:resource="http://purl.obolibrary.org/obo/OOSTT_00000083"/>
        <obo:IAO_0000115 xml:lang="en">An academic degree in the science and principles of nursing, granted by an accredited tertiary education provider after the successful completion of a bachelor&apos;s of nursing program.</obo:IAO_0000115>
        <obo:IAO_0000117 xml:lang="en">John Judkins</obo:IAO_0000117>
        <obo:IAO_0000117 xml:lang="en">Mathias Brochhausen</obo:IAO_0000117>
        <obo:IAO_0000119 xml:lang="en">https://en.wikipedia.org/w/index.php?title=Bachelor_of_Science_in_Nursing&amp;oldid=725962822</obo:IAO_0000119>
        <rdfs:label xml:lang="en">bachelor&apos;s of nursing degree</rdfs:label>
    </owl:Class>
    


    <!-- http://purl.obolibrary.org/obo/OOSTT_00000086 -->

    <owl:Class rdf:about="http://purl.obolibrary.org/obo/OOSTT_00000086">
        <rdfs:subClassOf rdf:resource="http://purl.obolibrary.org/obo/OOSTT_00000082"/>
        <obo:IAO_0000115 xml:lang="en">An academic degree in the science and principles of nursing, granted by an accredited tertiary education provider after the successful completion of a master&apos;s of nursing program.</obo:IAO_0000115>
        <obo:IAO_0000117 xml:lang="en">John Judkins</obo:IAO_0000117>
        <obo:IAO_0000117 xml:lang="en">Mathias Brochhausen</obo:IAO_0000117>
        <obo:OOSTT_00000030 xml:lang="en">An advanced academic degree in the principles and practices of nursing, with a focus on administration, education, or advanced nursing practice, granted by an accredited college or university after the successful completion of a master&apos;s of nursing program.</obo:OOSTT_00000030>
        <rdfs:label xml:lang="en">master&apos;s in the science of nursing degree</rdfs:label>
    </owl:Class>
</rdf:RDF>



<!-- Generated by the OWL API (version 4.5.6) https://github.com/owlcs/owlapi -->

